.

GIT.v
@@ -17,34 +17,69 @@ Lemma div_mod_uniqueness :
   a = b * q + r ->
   r < b ->
   a / b = q /\ a mod b = r.
-Proof.
+Proof with lia.
   assert (forall x : nat, forall y : nat, x > y <-> (exists z : nat, x = S (y + z))).
-  { intros x y; constructor.
-    - intros H; induction H.
-      + exists 0; lia.
-      + destruct IHle as [z H0]; exists (S z); lia.
-    - intros H; destruct H as [z H]; lia.
+  { intros x y. split.
+    - intros H. induction H.
+      + exists 0...
+      + destruct IHle as [z H0]; exists (S z)...
+    - intros H. destruct H as [z H]...
   }
   intros a b q r H1 H2.
-  assert (H0 : a = b * (a / b) + (a mod b)) by (apply (Nat.div_mod a b); lia).
-  assert (H3 : 0 <= a mod b < b).
-  { apply (Nat.mod_bound_pos a b).
-    - lia.
-    - lia.
-  }
+  assert (H0 : a = b * (a / b) + (a mod b)). { apply (Nat.div_mod a b)... }
+  assert (H3 : 0 <= a mod b < b). { apply (Nat.mod_bound_pos a b)... }
   assert (H4 : ~ q > a / b).
   { intros H4.
-    assert (H5 : exists z : nat, q = S (a / b + z)) by (apply (H q (a / b)); lia).
+    assert (H5 : exists z : nat, q = S (a / b + z)). { apply (H q (a / b))... }
     destruct H5 as [z H5].
-    cut (b * q + r >= b * S (a / b) + r); lia.
+    cut (b * q + r >= b * S (a / b) + r)...
   }
   assert (H5 : ~ q < a / b).
   { intros H5.
-    assert (H6 : exists z : nat, a / b = S (q + z)) by (apply (H (a / b) q); lia).
+    assert (H6 : exists z : nat, a / b = S (q + z)). { apply (H (a / b) q)... }
     destruct H6 as [z H6].
-    cut (b * q + a mod b >= b * S (a / b) + a mod b); lia.
+    cut (b * q + a mod b >= b * S (a / b) + a mod b)...
   }
-  assert (H6 : q = a / b) by lia; assert (H7 : r = a mod b) by lia; lia.
+  cut (q = a / b)...
+Qed.
+
+Fixpoint first_nat (p : nat -> bool) (n : nat) : nat :=
+  match n with
+  | 0 => 0
+  | S n' => if p (first_nat p n') then first_nat p n' else n
+  end
+.
+
+Theorem well_ordering_principle :
+  forall p : nat -> bool,
+  forall n : nat,
+  p n = true ->
+  let m := first_nat p n in
+  p m = true /\ (forall i : nat, p i = true -> i >= m).
+Proof with eauto. (* Improved By Clare Jang *)
+  intros p n H3 m.
+  assert (forall x : nat, p x = true -> p (first_nat p x) = true).
+  { induction x...
+    simpl.
+    destruct (p (first_nat p x)) eqn:H0...
+  }
+  split...
+  intros i H4.
+  enough (forall x : nat, first_nat p x <= x).
+  enough (forall x : nat, p (first_nat p x) = true -> (forall y : nat, x < y -> first_nat p x = first_nat p y)).
+  enough (forall x : nat, forall y : nat, p y = true -> first_nat p x <= y)...
+  - intros x y H2.
+    destruct (Compare_dec.le_lt_dec x y).
+    + eapply Nat.le_trans...
+    + replace (first_nat p x) with (first_nat p y)...
+  - intros x H1 y H2.
+    induction H2; simpl.
+    + rewrite H1...
+    + rewrite <- IHle.
+      rewrite H1...
+  - induction x...
+    simpl.
+    destruct (p (first_nat p x)) eqn: H0...
 Qed.
 
 Fixpoint sum_from_0_to (n : nat) : nat :=
@@ -57,10 +92,9 @@ Fixpoint sum_from_0_to (n : nat) : nat :=
 Theorem sum_from_0_to_is :
   forall n : nat,
   2 * sum_from_0_to n = n * (S n).
-Proof.
-  intros n; induction n.
-  - intuition.
-  - simpl in *; lia.
+Proof with eauto.
+  induction n; simpl in *...
+  lia.
 Qed.
 
 Fixpoint cantor_pairing (n : nat) : nat * nat :=
@@ -78,21 +112,24 @@ Lemma cantor_pairing_is_surjective :
   forall x : nat,
   forall y : nat,
   (x, y) = cantor_pairing (sum_from_0_to (x + y) + y).
-Proof.
-  cut (forall z : nat, forall y : nat, forall x : nat, z = x + y -> (x, y) = cantor_pairing (sum_from_0_to z + y)); eauto.
-  intros z; induction z.
-  - intros y x H; assert (H0 : x = 0) by lia; assert (H1 : y = 0) by lia; subst; eauto.
-  - intros y; induction y.
+Proof with (lia || eauto).
+  cut (forall z : nat, forall y : nat, forall x : nat, z = x + y -> (x, y) = cantor_pairing (sum_from_0_to z + y))...
+  induction z.
+  - intros y x H.
+    assert (H0 : x = 0)...
+    assert (H1 : y = 0)...
+    subst...
+  - induction y.
     + intros x H.
-      assert (H0 : x = S z) by lia.
-      subst; simpl cantor_pairing; destruct (cantor_pairing (z + sum_from_0_to z + 0)) eqn: H0.
-      assert (H1 : (0, z) = cantor_pairing (sum_from_0_to z + z)) by (apply IHz; reflexivity).
-      rewrite Nat.add_0_r in H0; rewrite Nat.add_comm in H0; rewrite H0 in H1.
-      inversion H1; subst; reflexivity.
+      assert (H0 : x = S z)... subst. simpl.
+      destruct (cantor_pairing (z + sum_from_0_to z + 0)) eqn: H0.
+      assert (H1 : (0, z) = cantor_pairing (sum_from_0_to z + z))...
+      rewrite Nat.add_0_r in H0. rewrite Nat.add_comm in H0. rewrite H0 in H1.
+      inversion H1. subst...
     + intros x H.
-      assert (H0 : (S x, y) = cantor_pairing (sum_from_0_to (S z) + y)) by (apply (IHy (S x)); lia).
-      assert (H1 : z + sum_from_0_to z + S y = sum_from_0_to (S z) + y) by (simpl; lia).
-      simpl; rewrite H1; rewrite <- H0; eauto.
+      assert (H0 : (S x, y) = cantor_pairing (sum_from_0_to (S z) + y)). { apply (IHy (S x))... }
+      assert (H1 : z + sum_from_0_to z + S y = sum_from_0_to (S z) + y). { simpl... }
+      simpl. rewrite H1. rewrite <- H0...
 Qed.
 
 Lemma cantor_pairing_is_injective :
@@ -101,43 +138,45 @@ Lemma cantor_pairing_is_injective :
   forall y : nat,
   cantor_pairing n = (x, y) ->
   n = sum_from_0_to (x + y) + y.
-Proof.
-  intros n; induction n.
-  - simpl; intros x y H; inversion H; subst; reflexivity.
-  - simpl; intros x y H; destruct (cantor_pairing n) as [x' y'] eqn: H0; destruct x'.
-    + inversion H; subst; repeat (rewrite Nat.add_0_r); simpl; rewrite (IHn 0 y' eq_refl); rewrite Nat.add_0_l; lia.
-    + inversion H; subst; rewrite (IHn (S x) y' eq_refl); assert (H1 : forall x' : nat, S x' + y' = x' + S y') by lia; repeat (rewrite H1); lia.
+Proof with (lia || eauto).
+  induction n; simpl.
+  - intros x y H.
+    inversion H. subst...
+  - intros x y H.
+    destruct (cantor_pairing n) as [x' y'] eqn: H0.
+    destruct x'; (inversion H; subst).
+    + repeat (rewrite Nat.add_0_r).
+      simpl.
+      rewrite (IHn 0 y' eq_refl).
+      rewrite Nat.add_0_l...
+    + rewrite (IHn (S x) y' eq_refl).
+      assert (H1 : forall x' : nat, S x' + y' = x' + S y')...
+      repeat (rewrite H1)...
 Qed.
 
-Theorem cantor_pairing_is :
+Lemma cantor_pairing_is :
   forall n : nat,
   forall x : nat,
   forall y : nat,
   cantor_pairing n = (x, y) <-> n = sum_from_0_to (x + y) + y.
 Proof.
-  intros n x y; constructor.
-  - apply (cantor_pairing_is_injective n x y).
-  - intros H; subst; rewrite (cantor_pairing_is_surjective x y); reflexivity.
+  intros n x y. split; [apply (cantor_pairing_is_injective n x y) | intros; subst; eauto using (cantor_pairing_is_surjective x y)].
 Qed.
 
 Lemma forallb_true_iff {A : Type} (f : A -> bool) :
   forall xs : list A,
   forallb f xs = true <-> (forall x : A, In x xs -> f x = true).
-Proof.
-  intros xs; induction xs as [| x' xs].
-  - simpl; constructor.
-    + intros H x H0; contradiction.
-    + tauto.
-  - simpl; rewrite andb_true_iff; constructor.
-    + intros H; destruct H as [H H0]; intros x H1; destruct H1.
-      * subst; apply H.
-      * apply IHxs.
-        apply H0.
-        apply H1.
-    + intros H; constructor.
-      * apply H; left; reflexivity.
-      * apply IHxs.
-        intros x H0; apply H; right; apply H0.
+Proof with eauto.
+  intros xs; induction xs as [| x' xs]; simpl.
+  - split; [contradiction | tauto].
+  - rewrite andb_true_iff. split.
+    + intros H.
+      destruct H as [H H0].
+      intros x H1.
+      destruct H1; [subst | apply IHxs]...
+    + intros H.
+      split...
+      apply IHxs...
 Qed.
 
 Definition fold_right_max_0 : list nat -> nat :=
@@ -149,22 +188,23 @@ Lemma fold_right_max_0_in :
   forall n : nat,
   In n ns ->
   fold_right_max_0 ns >= n.
-Proof.
-  unfold fold_right_max_0; intros ns; induction ns as [| n' ns].
-  - simpl; lia.
-  - simpl; intros n H; destruct H.
-    + lia.
-    + assert (fold_right max 0 ns >= n) by (apply IHns; apply H); lia.
+Proof with (lia || eauto).
+  unfold fold_right_max_0.
+  induction ns as [| n' ns]; simpl...
+  intros n H.
+  destruct H...
+  enough (fold_right max 0 ns >= n)...
 Qed.
 
 Lemma fold_right_max_0_app :
   forall ns1 : list nat,
   forall ns2 : list nat,
   fold_right_max_0 (ns1 ++ ns2) = max (fold_right_max_0 ns1) (fold_right_max_0 ns2).
-Proof.
-  unfold fold_right_max_0; intros ns1; induction ns1 as [|n1 ns1].
-  - simpl; intros n; lia.
-  - simpl; intros n; rewrite IHns1; lia.
+Proof with (lia || eauto).
+  unfold fold_right_max_0.
+  induction ns1 as [|n1 ns1]; simpl... 
+  intros n.
+  rewrite IHns1...
 Qed.
 
 Definition ensemble (A : Type) : Type :=
@@ -228,7 +268,9 @@ Lemma isSubsetOf_refl {A : Type} :
   forall xs1 : ensemble A,
   isSubsetOf xs1 xs1.
 Proof.
-  unfold isSubsetOf; intros xs1 x H; apply H.
+  unfold isSubsetOf.
+  intros xs1 x H.
+  apply H.
 Qed.
 
 Lemma isSubsetOf_trans {A : Type} :
@@ -239,7 +281,9 @@ Lemma isSubsetOf_trans {A : Type} :
   isSubsetOf xs2 xs3 ->
   isSubsetOf xs1 xs3.
 Proof.
-  unfold isSubsetOf; intros xs1 xs2 xs3 H1 H2; apply (fun x : A => fun H0 : member x xs1 => H2 x (H1 x H0)).
+  unfold isSubsetOf.
+  intros xs1 xs2 xs3 H1 H2.
+  apply (fun x : A => fun H0 : member x xs1 => H2 x (H1 x H0)).
 Qed.
 
 End Preliminaries.
@@ -271,8 +315,8 @@ Lemma diagonalizer_diagonalizes (mathcalE : Type) `{mathcalE_is_goedelian : Goed
   forall E : mathcalE,
   enum_mathcalE n = E ->
   enum_mathcalE (diagonalizer mathcalE n) = apply_nat E n.
-Proof.
-  intros n E H; unfold diagonalizer; subst; destruct (mathcalE_is_denumerable (apply_nat (enum_mathcalE n) n)) as [d_n]; simpl; tauto.
+Proof with eauto.
+  unfold diagonalizer. intros. subst. destruct (mathcalE_is_denumerable (apply_nat (enum_mathcalE n) n)) as [d_n]...
 Qed.
 
 Definition expressPredicate (mathcalE : Type) `{mathcalE_is_goedelian : GoedelianLanguage mathcalE} : mathcalE -> ensemble nat -> Prop :=
@@ -306,32 +350,33 @@ Theorem After_Goedel_with_shades_of_Tarski (mathcalE : Type) `{mathcalE_is_goede
   isCorrect mathcalE ->
   is_expressible mathcalE (StarOf mathcalE (completement (P mathcalE))) ->
   exists E : mathcalE, isTrue E /\ ~ isProvable E.
-Proof.
+Proof with eauto.
   intros mathcalE_is_correct StarOf_complement_P_is_expressible.
   destruct StarOf_complement_P_is_expressible as [H H_express_StarOf_complement_P].
   destruct (mathcalE_is_denumerable H) as [n n_is_the_goedel_number_of_H].
   assert (diagonalization_of_n_is_true_iff_n_is_in_StarOf_complement_of_P : isTrue (enum_mathcalE (diagonalizer mathcalE n)) <-> member n (StarOf mathcalE (completement (P mathcalE)))).
   { unfold expressPredicate in H_express_StarOf_complement_P.
-    rewrite (diagonalizer_diagonalizes mathcalE n H n_is_the_goedel_number_of_H).
-    apply H_express_StarOf_complement_P.
+    rewrite (diagonalizer_diagonalizes mathcalE n H n_is_the_goedel_number_of_H)...
   }
   assert (n_in_StarOf_complement_of_P_iff_diagonalization_of_n_is_not_Provable : member n (StarOf mathcalE (completement (P mathcalE))) <-> ~ isProvable (enum_mathcalE (diagonalizer mathcalE n))).
-  { constructor.
+  { split.
     - intros n_in_StarOf_complement_of_P diagonalization_of_n_is_not_Provable.
-      inversion n_in_StarOf_complement_of_P as [A n' diagonalization_of_n_is_in_A A_is_complement_of_P n_is_n']; subst n'; contradiction diagonalization_of_n_is_in_A.
-      apply InP; apply diagonalization_of_n_is_not_Provable.
-    - intros diagonalization_of_n_is_not_Provable; apply InStarOf.
-      intros diagonalization_of_n_is_in_P; contradiction diagonalization_of_n_is_not_Provable.
-      inversion diagonalization_of_n_is_in_P as [n' diagonalization_of_n_is_Provable n_is_n']; subst n'; apply diagonalization_of_n_is_Provable.
+      inversion n_in_StarOf_complement_of_P as [A n' diagonalization_of_n_is_in_A A_is_complement_of_P n_is_n']; subst n'.
+      contradiction diagonalization_of_n_is_in_A.
+      constructor...
+    - intros diagonalization_of_n_is_not_Provable.
+      constructor.
+      intros diagonalization_of_n_is_in_P.
+      contradiction diagonalization_of_n_is_not_Provable.
+      inversion diagonalization_of_n_is_in_P as [n' diagonalization_of_n_is_Provable n_is_n']; subst n'...
   }
   assert (diagonalization_of_n_is_not_Provable : ~ isProvable (enum_mathcalE (diagonalizer mathcalE n))).
   { intros diagonalization_of_n_is_Provable.
     destruct mathcalE_is_correct as [Provable_implies_true Refutable_implies_false].
-    assert (diagonalization_of_n_is_True : isTrue (enum_mathcalE (diagonalizer mathcalE n))) by (apply Provable_implies_true; apply diagonalization_of_n_is_Provable).
+    assert (diagonalization_of_n_is_True : isTrue (enum_mathcalE (diagonalizer mathcalE n))) by firstorder.
     tauto.
   }
-  exists (enum_mathcalE (diagonalizer mathcalE n)).
-  tauto.
+  firstorder.
 Qed.
 
 Definition the_first_goal (mathcalE : Type) `{mathcalE_is_goedelian : GoedelianLanguage mathcalE} : Prop :=
@@ -354,19 +399,26 @@ Lemma A_Diagonal_Lemma_a (mathcalE : Type) `{mathcalE_is_goedelian : GoedelianLa
   forall A : ensemble nat,
   is_expressible mathcalE (StarOf mathcalE A) ->
   exists E : mathcalE, isGoedelSentence mathcalE E A.
-Proof.
-  intros A StarOf_A_is_expressible; destruct StarOf_A_is_expressible as [H H_express_StarOf_A]; destruct (mathcalE_is_denumerable H) as [n g_H_is_n]; exists (apply_nat H n).
-  assert (isTrue (apply_nat H n) <-> member (diagonalizer mathcalE n) A).
-  { constructor.
-    - intros H_n_is_true; assert (n_is_in_StarOfA : member n (StarOf mathcalE A)) by (apply H_express_StarOf_A; apply H_n_is_true).
-      inversion n_is_in_StarOfA as [A' n' d_n_is_in_A A_is_A' n_is_n']; subst; apply d_n_is_in_A.
-    - intros d_n_is_in_A; apply H_express_StarOf_A; constructor; apply d_n_is_in_A.
+Proof with eauto.
+  intros A StarOf_A_is_expressible.
+  destruct StarOf_A_is_expressible as [H H_express_StarOf_A].
+  destruct (mathcalE_is_denumerable H) as [n g_H_is_n].
+  exists (apply_nat H n).
+  assert (H_n_is_true_iff_d_n_is_in_A : isTrue (apply_nat H n) <-> member (diagonalizer mathcalE n) A).
+  { split.
+    - intros H_n_is_true.
+      assert (n_is_in_StarOfA : member n (StarOf mathcalE A)) by firstorder.
+      inversion n_is_in_StarOfA as [A' n' d_n_is_in_A A_is_A' n_is_n']; subst...
+    - intros d_n_is_in_A.
+      apply H_express_StarOf_A.
+      constructor...
   }
-  assert (enum_mathcalE (diagonalizer mathcalE n) = apply_nat H n).
-  { unfold diagonalizer; rewrite (proj2_sig (mathcalE_is_denumerable (apply_nat (enum_mathcalE n) n))).
-    rewrite g_H_is_n; reflexivity.
+  assert (d_n_is_g_H_n : enum_mathcalE (diagonalizer mathcalE n) = apply_nat H n).
+  { unfold diagonalizer.
+    rewrite (proj2_sig (mathcalE_is_denumerable (apply_nat (enum_mathcalE n) n))).
+    rewrite g_H_is_n...
   }
-  exists (diagonalizer mathcalE n); tauto.
+  firstorder.
 Qed.
 
 Lemma A_Diagonal_Lemma_b (mathcalE : Type) `{mathcalE_is_goedelian : GoedelianLanguage mathcalE} :
@@ -374,8 +426,10 @@ Lemma A_Diagonal_Lemma_b (mathcalE : Type) `{mathcalE_is_goedelian : GoedelianLa
   forall A : ensemble nat,
   is_expressible mathcalE A ->
   exists E : mathcalE, isGoedelSentence mathcalE E A.
-Proof.
-  intros the_first_goal_holds A A_is_expressible; apply A_Diagonal_Lemma_a; apply the_first_goal_holds; apply A_is_expressible.
+Proof with eauto.
+  intros the_first_goal_holds A A_is_expressible.
+  apply A_Diagonal_Lemma_a.
+  apply the_first_goal_holds...
 Qed.
 
 Inductive T (mathcalE : Type) `{mathcalE_is_goedelian : GoedelianLanguage mathcalE} : ensemble nat :=
@@ -387,44 +441,48 @@ Inductive T (mathcalE : Type) `{mathcalE_is_goedelian : GoedelianLanguage mathca
 
 Theorem there_is_no_GoedelSentence_of_complement_of_T (mathcalE : Type) `{mathcalE_is_goedelian : GoedelianLanguage mathcalE} :
   ~ exists E : mathcalE, isGoedelSentence mathcalE E (completement (T mathcalE)).
-Proof.
+Proof with (tauto || eauto).
   intros there_is_GoedelSentence_of_complement_of_T.
   destruct there_is_GoedelSentence_of_complement_of_T as [E E_is_GoedelSentence_of_complement_of_T].
   destruct E_is_GoedelSentence_of_complement_of_T as [n n_is_g_E_and_E_is_true_iff_n_is_in_complement_T].
   destruct n_is_g_E_and_E_is_true_iff_n_is_in_complement_T as [n_is_g_E E_is_true_iff_n_is_in_complement_T].
-  assert (E_is_true_iff_n_is_not_in_T : isTrue E <-> ~ member n (T mathcalE)) by (rewrite E_is_true_iff_n_is_in_complement_T; unfold completement; unfold member; reflexivity).
-  assert (E_is_true_iff_n_is_in_T : isTrue E <-> member n (T mathcalE)).
-  { constructor.
-    - intros E_is_true; constructor; rewrite n_is_g_E; apply E_is_true.
-    - intros n_is_inT; inversion n_is_inT as [n' E_is_true n_is_n']; subst n'; rewrite <- n_is_g_E; apply E_is_true.
-  }
-  tauto.
+  assert (E_is_true_iff_n_is_not_in_T : isTrue E <-> ~ member n (T mathcalE)) by firstorder.
+  assert (E_is_true_iff_n_is_in_T : isTrue E <-> member n (T mathcalE))...
+  split.
+  - intros E_is_true.
+    constructor.
+    rewrite n_is_g_E...
+  - intros n_is_inT.
+    inversion n_is_inT as [n' E_is_true n_is_n']; subst n'.
+    rewrite <- n_is_g_E...
 Qed.
 
 Theorem After_Tarski_1 (mathcalE : Type) `{mathcalE_is_goedelian : GoedelianLanguage mathcalE} :
   ~ is_expressible mathcalE (StarOf mathcalE (completement (T mathcalE))).
-Proof.
+Proof with eauto.
   intros StarOf_T_is_expressible.
   destruct (A_Diagonal_Lemma_a mathcalE (completement (T mathcalE)) StarOf_T_is_expressible) as [H H_is_GoedelSentence_for_complement_of_T].
   contradiction (there_is_no_GoedelSentence_of_complement_of_T mathcalE).
-  exists H; apply H_is_GoedelSentence_for_complement_of_T.
+  exists H...
 Qed.
 
 Theorem After_Tarski_2 (mathcalE : Type) `{mathcalE_is_goedelian : GoedelianLanguage mathcalE} :
   the_first_goal mathcalE ->
   ~ is_expressible mathcalE (completement (T mathcalE)).
-Proof.
+Proof with eauto.
   intros the_first_goal_holds completement_of_T_is_expressible.
-  apply (After_Tarski_1 mathcalE); apply the_first_goal_holds; apply completement_of_T_is_expressible.
+  apply (After_Tarski_1 mathcalE).
+  apply the_first_goal_holds...
 Qed.
 
 Theorem After_Tarski_3 (mathcalE : Type) `{mathcalE_is_goedelian : GoedelianLanguage mathcalE} :
   the_first_goal mathcalE ->
   the_second_goal mathcalE ->
   ~ is_expressible mathcalE (T mathcalE).
-Proof.
+Proof with eauto.
   intros the_first_goal_holds the_second_goal_holds T_is_expressible.
-  apply (After_Tarski_2 mathcalE the_first_goal_holds); apply the_second_goal_holds; apply T_is_expressible.
+  apply (After_Tarski_2 mathcalE the_first_goal_holds).
+  apply the_second_goal_holds...
 Qed.
 
 End Chapter1.
@@ -496,29 +554,20 @@ Theorem the_rule_of_getFreeVars_tm :
   forall t : tm,
   forall x : vr,
   In x (getFreeVars_tm t) <-> occursFreeIn_tm x t = true.
-Proof.
-  intros t; induction t.
-  - intros vr; simpl; constructor.
-    + intros H; destruct H.
-      { subst.
-        destruct (vr_eq_dec vr vr).
-        - reflexivity.
-        - contradiction.
-      }
-      { contradiction.
-      }
-    + intros H; destruct (vr_eq_dec vr v).
-      { rewrite e; left; reflexivity.
-      }
-      { inversion H.
-      }
-  - intros vr; simpl; constructor.
-    + tauto.
-    + intros H; inversion H.
-  - intros vr; simpl; apply IHt.
-  - intros vr; simpl; rewrite orb_true_iff; rewrite in_app_iff; rewrite IHt1; rewrite IHt2; reflexivity.
-  - intros vr; simpl; rewrite orb_true_iff; rewrite in_app_iff; rewrite IHt1; rewrite IHt2; reflexivity.
-  - intros vr; simpl; rewrite orb_true_iff; rewrite in_app_iff; rewrite IHt1; rewrite IHt2; reflexivity.
+Proof with eauto.
+  induction t; simpl; [> (intros vr; simpl; rewrite orb_true_iff; rewrite in_app_iff; rewrite IHt1; rewrite IHt2; reflexivity) || eauto ..].
+  - intros vr.
+    split.
+    + intros H.
+      destruct H...
+      subst.
+      destruct (vr_eq_dec vr vr)...
+    + intros H.
+      destruct (vr_eq_dec vr v)...
+      inversion H.
+  - split...
+    intros H.
+    inversion H.
 Qed.
 
 Fixpoint getFreeVars_form (f : form) : list vr :=
@@ -535,29 +584,31 @@ Theorem the_rule_of_getFreeVars_form :
   forall f : form,
   forall x : vr,
   In x (getFreeVars_form f) <-> occursFreeIn_form x f = true.
-Proof.
-  intros f; induction f.
-  - intros vr; simpl; rewrite orb_true_iff; rewrite in_app_iff; rewrite the_rule_of_getFreeVars_tm; rewrite the_rule_of_getFreeVars_tm; reflexivity.
-  - intros vr; simpl; rewrite orb_true_iff; rewrite in_app_iff; rewrite the_rule_of_getFreeVars_tm; rewrite the_rule_of_getFreeVars_tm; reflexivity.
-  - intros vr; simpl; apply IHf.
-  - intros vr; simpl; rewrite orb_true_iff; rewrite in_app_iff; rewrite IHf1; rewrite IHf2; reflexivity.
-  - intros vr; simpl; constructor.
+Proof with (reflexivity || eauto).
+  intros f; induction f; simpl...
+  - intros.
+    rewrite orb_true_iff.
+    rewrite in_app_iff.
+    repeat (rewrite the_rule_of_getFreeVars_tm)...
+  - intros.
+    rewrite orb_true_iff.
+    rewrite in_app_iff.
+    repeat (rewrite the_rule_of_getFreeVars_tm)...
+  - intros.
+    rewrite orb_true_iff.
+    rewrite in_app_iff.
+    rewrite IHf1.
+    rewrite IHf2...
+  - intros.
+    split.
     + intros H.
-      assert (In vr (getFreeVars_form f) /\ vr <> v).
-      { apply (in_remove vr_eq_dec (getFreeVars_form f) vr v); apply H.
-      }
-      destruct H0 as [H0 H1]; destruct (vr_eq_dec vr v).
-      { contradiction H1.
-      }
-      { apply IHf; apply H0.
-      }
-    + intros H; destruct (vr_eq_dec vr v).
-      { inversion H.
-      }
-      { apply in_in_remove.
-        - apply n.
-        - apply IHf; apply H.
-      }
+      assert (In x (getFreeVars_form f) /\ x <> v) by now apply (in_remove vr_eq_dec (getFreeVars_form f) x v).
+      destruct H0 as [H0 H1].
+      destruct (vr_eq_dec x v)...
+      apply IHf...
+    + intros H.
+      destruct (vr_eq_dec x v); [inversion H | apply in_in_remove]...
+      apply IHf...
 Qed.
 
 Definition value_assignment : Set :=
@@ -581,35 +632,23 @@ Lemma eval_tm_extensionality :
   forall va2 : value_assignment,
   (forall x : vr, occursFreeIn_tm x t = true -> va1 x = va2 x) ->
   eval_tm va1 t = eval_tm va2 t.
-Proof.
-  intros t; induction t.
-  - simpl; intros va1 va2 H; apply H; destruct (vr_eq_dec v v).
-    + reflexivity.
-    + contradiction.
-  - simpl; intros va1 va2 H.
-    reflexivity.
-  - simpl; intros va1 va2 H.
-    rewrite (IHt va1 va2).
-    reflexivity.
+Proof with eauto.
+  induction t; simpl...
+  - intros va1 va2 H.
     apply H.
-  - simpl; intros va1 va2 H.
-    rewrite (IHt1 va1 va2).
-    rewrite (IHt2 va1 va2).
+    destruct (vr_eq_dec v v)...
+  - intros va1 va2 H.
+    rewrite (IHt1 va1 va2); [ | intros x H0; apply H; apply orb_true_iff; tauto].
+    rewrite (IHt2 va1 va2); [ | intros x H0; apply H; apply orb_true_iff; tauto].
     reflexivity.
-    intros x H0; apply H; apply orb_true_iff; tauto.
-    intros x H0; apply H; apply orb_true_iff; tauto.
-  - simpl; intros va1 va2 H.
-    rewrite (IHt1 va1 va2).
-    rewrite (IHt2 va1 va2).
+  - intros va1 va2 H.
+    rewrite (IHt1 va1 va2); [ | intros x H0; apply H; apply orb_true_iff; tauto].
+    rewrite (IHt2 va1 va2); [ | intros x H0; apply H; apply orb_true_iff; tauto].
     reflexivity.
-    intros x H0; apply H; apply orb_true_iff; tauto.
-    intros x H0; apply H; apply orb_true_iff; tauto.
-  - simpl; intros va1 va2 H.
-    rewrite (IHt1 va1 va2).
-    rewrite (IHt2 va1 va2).
+  - intros va1 va2 H.
+    rewrite (IHt1 va1 va2); [ | intros x H0; apply H; apply orb_true_iff; tauto].
+    rewrite (IHt2 va1 va2); [ | intros x H0; apply H; apply orb_true_iff; tauto].
     reflexivity.
-    intros x H0; apply H; apply orb_true_iff; tauto.
-    intros x H0; apply H; apply orb_true_iff; tauto.
 Qed.
 
 Fixpoint eval_form (va : value_assignment) (f : form) : Prop :=
@@ -628,50 +667,35 @@ Lemma eval_form_extensionality :
   forall va2 : value_assignment,
   (forall x : vr, occursFreeIn_form x f = true -> va1 x = va2 x) ->
   eval_form va1 f <-> eval_form va2 f.
-Proof.
-  intros f; induction f.
-  - simpl; intros va1 va2 H.
-    rewrite (eval_tm_extensionality t va1 va2).
-    rewrite (eval_tm_extensionality t0 va1 va2).
+Proof with eauto.
+  induction f; simpl...
+  - intros va1 va2 H.
+    rewrite (eval_tm_extensionality t va1 va2); [ | intros x H0; apply H; apply orb_true_iff]...
+    rewrite (eval_tm_extensionality t0 va1 va2); [ | intros x H0; apply H; apply orb_true_iff]...
     reflexivity.
-    intros x H0; apply H; apply orb_true_iff; tauto.
-    intros x H0; apply H; apply orb_true_iff; tauto.
-  - simpl; intros va1 va2 H.
-    rewrite (eval_tm_extensionality t va1 va2).
-    rewrite (eval_tm_extensionality t0 va1 va2).
+  - intros va1 va2 H.
+    rewrite (eval_tm_extensionality t va1 va2); [ | intros x H0; apply H; apply orb_true_iff]...
+    rewrite (eval_tm_extensionality t0 va1 va2); [ | intros x H0; apply H; apply orb_true_iff]...
     reflexivity.
-    intros x H0; apply H; apply orb_true_iff; tauto.
-    intros x H0; apply H; apply orb_true_iff; tauto.
-  - simpl; intros va1 va2 H.
-    rewrite (IHf va1 va2).
+  - intros va1 va2 H.
+    rewrite (IHf va1 va2); [ | intros x H0; apply H]...
     reflexivity.
-    intros x H0; apply H; tauto.
-  - simpl; intros va1 va2 H.
-    rewrite (IHf1 va1 va2).
-    rewrite (IHf2 va1 va2).
+  - intros va1 va2 H.
+    rewrite (IHf1 va1 va2); [ | intros x H0; apply H; apply orb_true_iff]...
+    rewrite (IHf2 va1 va2); [ | intros x H0; apply H; apply orb_true_iff]...
     reflexivity.
-    intros x H0; apply H; apply orb_true_iff; tauto.
-    intros x H0; apply H; apply orb_true_iff; tauto.
-  - simpl; intros va1 va2 H.
+  - intros va1 va2 H.
     cut (
       forall n : nat,
       eval_form (fun z : vr => if vr_eq_dec v z then n else va1 z) f <->  eval_form (fun z : vr => if vr_eq_dec v z then n else va2 z) f
     ).
-    { constructor.
-      - intros H1 n; apply H0; apply H1.
-      - intros H1 n; apply H0; apply H1.
-    }
+      firstorder.
     intros n.
-    rewrite (IHf (fun z : vr => if vr_eq_dec v z then n else va1 z) (fun z : vr => if vr_eq_dec v z then n else va2 z)).
-    reflexivity.
-    intros x H0; destruct (vr_eq_dec v x).
-    { reflexivity.
-    }
-    { apply H.
-      destruct (vr_eq_dec x v).
-      - contradiction n0; rewrite e; reflexivity.
-      - apply H0.
-    }
+    rewrite (IHf (fun z : vr => if vr_eq_dec v z then n else va1 z) (fun z : vr => if vr_eq_dec v z then n else va2 z))...
+    intros x H0.
+    destruct (vr_eq_dec v x)...
+    apply H.
+    destruct (vr_eq_dec x v)...
 Qed.
 
 Fixpoint make_numeral (n : nat) : tm :=
@@ -685,10 +709,8 @@ Lemma eval_tm_make_numeral :
   forall n : nat,
   forall va : value_assignment,
   eval_tm va (make_numeral n) = n.
-Proof.
-  intros n; induction n.
-  - simpl; intros va; reflexivity.
-  - simpl; intros va; rewrite IHn; reflexivity.
+Proof with eauto.
+  induction n; simpl...
 Qed.
 
 Definition substitution : Set :=
@@ -718,14 +740,8 @@ Theorem substitute_tm_preserves_eval_tm :
   forall sigma : substitution,
   forall va : value_assignment,
   eval_tm (fun z : vr => eval_tm va (substitute_vr sigma z)) t = eval_tm va (substitute_tm sigma t).
-Proof.
-  intros t; induction t.
-  - intros sigma va; simpl; reflexivity.
-  - intros sigma va; simpl; reflexivity.
-  - intros sigma va; simpl; rewrite IHt; reflexivity.
-  - intros sigma va; simpl; rewrite IHt1; rewrite IHt2; reflexivity.
-  - intros sigma va; simpl; rewrite IHt1; rewrite IHt2; reflexivity.
-  - intros sigma va; simpl; rewrite IHt1; rewrite IHt2; reflexivity.
+Proof with eauto.
+  induction t; simpl...
 Qed.
 
 Definition getMaxNumOfFreeVars_tm (t : tm) : vr :=
@@ -736,22 +752,23 @@ Lemma getMaxNumOfFreeVars_tm_lt :
   forall x : vr,
   getMaxNumOfFreeVars_tm t < x ->
   occursFreeIn_tm x t = false.
-Proof.
-  unfold getMaxNumOfFreeVars_tm; intros t; induction t.
-  - simpl; intros x H; destruct (vr_eq_dec x v).
-    + lia.
-    + reflexivity.
-  - simpl; intros x H; tauto.
-  - simpl; intros x H; apply IHt; apply H.
-  - simpl; intros x H; apply orb_false_iff; rewrite fold_right_max_0_app in H; constructor.
-    + apply IHt1; lia.
-    + apply IHt2; lia.
-  - simpl; intros x H; apply orb_false_iff; rewrite fold_right_max_0_app in H; constructor.
-    + apply IHt1; lia.
-    + apply IHt2; lia.
-  - simpl; intros x H; apply orb_false_iff; rewrite fold_right_max_0_app in H; constructor.
-    + apply IHt1; lia.
-    + apply IHt2; lia.
+Proof with eauto.
+  unfold getMaxNumOfFreeVars_tm.
+  induction t; simpl...
+  - intros x H.
+    destruct (vr_eq_dec x v); [lia | reflexivity].
+  - intros x H.
+    apply orb_false_iff.
+    rewrite fold_right_max_0_app in H.
+    split; [apply IHt1; lia | apply IHt2; lia].
+  - intros x H.
+    apply orb_false_iff.
+    rewrite fold_right_max_0_app in H.
+    split; [apply IHt1; lia | apply IHt2; lia].
+  - intros x H.
+    apply orb_false_iff.
+    rewrite fold_right_max_0_app in H.
+    split; [apply IHt1; lia | apply IHt2; lia].
 Qed.
 
 Definition isFreshVarIn_substitute_tm (sigma : substitution) (z : vr) (t : tm) : Prop :=
@@ -770,7 +787,7 @@ Theorem the_rule_of_chi :
   forall f : form,
   forall sigma : substitution,
   isFreshVarIn_substitute_form sigma (chi sigma f) f.
-Proof.
+Proof with eauto.
   assert ( claim1 :
     forall sigma : substitution,
     forall f : form,
@@ -780,20 +797,24 @@ Proof.
   ).
   { intros sigma f x H.
     assert (getMaxNumOfFreeVars_tm (substitute_vr sigma x) < chi sigma f).
-    { unfold chi; unfold fold_right_max_0.
-      cut (fold_right max 0 (map (fun z : vr => getMaxNumOfFreeVars_tm (substitute_vr sigma z)) (getFreeVars_form f)) >= getMaxNumOfFreeVars_tm (substitute_vr sigma x)).
-      { lia.
-      }
+    { unfold chi.
+      unfold fold_right_max_0.
+      cut (fold_right max 0 (map (fun z : vr => getMaxNumOfFreeVars_tm (substitute_vr sigma z)) (getFreeVars_form f)) >= getMaxNumOfFreeVars_tm (substitute_vr sigma x)); [lia | ].
       rewrite <- the_rule_of_getFreeVars_form in H.
-      apply fold_right_max_0_in; apply in_map_iff.
-      exists x; constructor.
-      - reflexivity.
-      - apply H.
+      apply fold_right_max_0_in.
+      apply in_map_iff.
+      exists x.
+      split...
     }
-    apply getMaxNumOfFreeVars_tm_lt; apply H0.
+    apply getMaxNumOfFreeVars_tm_lt...
   }
-  unfold isFreshVarIn_substitute_form; intros f sigma; apply forallb_true_iff.
-  intros x H; apply negb_true_iff; apply claim1; apply the_rule_of_getFreeVars_form; apply H.
+  unfold isFreshVarIn_substitute_form.
+  intros f sigma.
+  apply forallb_true_iff.
+  intros x H.
+  apply negb_true_iff.
+  apply claim1.
+  apply the_rule_of_getFreeVars_form...
 Qed.
 
 Fixpoint substitute_form (sigma : substitution) (f : form) : form :=
@@ -813,59 +834,64 @@ Theorem substitute_form_preserves_eval_form :
   forall sigma : substitution,
   forall va : value_assignment,
   eval_form (fun z : vr => eval_tm va (substitute_vr sigma z)) f <-> eval_form va (substitute_form sigma f).
-Proof.
-  intros f; induction f.
-  - intros sigma va; simpl.
-    rewrite substitute_tm_preserves_eval_tm; rewrite substitute_tm_preserves_eval_tm; reflexivity.
-  - intros sigma va; simpl.
-    rewrite substitute_tm_preserves_eval_tm; rewrite substitute_tm_preserves_eval_tm; reflexivity.
-  - intros sigma va; simpl.
-    rewrite IHf; reflexivity.
-  - intros sigma va; simpl.
-    rewrite IHf1; rewrite IHf2; reflexivity.
-  - intros sigma va. simpl.
-    cut (
+Proof with (reflexivity || eauto).
+  induction f; simpl...
+  - intros sigma va.
+    repeat (rewrite substitute_tm_preserves_eval_tm)...
+  - intros sigma va.
+    repeat (rewrite substitute_tm_preserves_eval_tm)...
+  - intros sigma va.
+    rewrite IHf...
+  - intros sigma va.
+    rewrite IHf1.
+    rewrite IHf2...
+  - intros sigma va.
+    assert ( claim1 :
       forall n : nat,
       eval_form (fun z : vr => if vr_eq_dec v z then n else eval_tm va (substitute_vr sigma z)) f <-> eval_form (fun z : vr => if vr_eq_dec (chi sigma (all_form v f)) z then n else va z) (substitute_form ((v, ivar_tm (chi sigma (all_form v f))) :: sigma) f)
     ).
-    { intros H; constructor.
-      - intros H0 n; apply H; apply H0.
-      - intros H0 n; apply H; apply H0.
-    }
-    intros n; rewrite <- (IHf ((v, ivar_tm (chi sigma (all_form v f))) :: sigma) (fun z : vr => if vr_eq_dec (chi sigma (all_form v f)) z then n else va z)); apply eval_form_extensionality.
-    intros x H; simpl; destruct (vr_eq_dec v x).
-    { destruct (vr_eq_dec x v).
-      - simpl; destruct (vr_eq_dec (chi sigma (all_form v f)) (chi sigma (all_form v f))).
-        + reflexivity.
-        + contradiction.
-      - contradiction n0; rewrite e; reflexivity.
-    }
-    { destruct (vr_eq_dec x v).
-      - contradiction n0; rewrite e; reflexivity.
-      - apply eval_tm_extensionality.
-        intros x' H0; destruct (vr_eq_dec (chi sigma (all_form v f)) x').
-        + subst.
-          assert (isFreshVarIn_substitute_form sigma (chi sigma (all_form v f)) (all_form v f)).
-            apply the_rule_of_chi.
-          unfold isFreshVarIn_substitute_form in H1; rewrite forallb_true_iff in H1.
+    { intros n.
+      rewrite <- (IHf ((v, ivar_tm (chi sigma (all_form v f))) :: sigma) (fun z : vr => if vr_eq_dec (chi sigma (all_form v f)) z then n else va z)).
+      apply eval_form_extensionality.
+      intros x H.
+      simpl.
+      destruct (vr_eq_dec v x).
+      { destruct (vr_eq_dec x v).
+        - simpl.
+          destruct (vr_eq_dec (chi sigma (all_form v f)) (chi sigma (all_form v f)))...
+          contradiction.
+        - contradiction n0...
+      }
+      { destruct (vr_eq_dec x v).
+        - contradiction n0...
+        - apply eval_tm_extensionality.
+          intros x' H0.
+          destruct (vr_eq_dec (chi sigma (all_form v f)) x')...
+          subst.
+          assert (isFreshVarIn_substitute_form sigma (chi sigma (all_form v f)) (all_form v f)) by apply the_rule_of_chi.
+          unfold isFreshVarIn_substitute_form in H1.
+          rewrite forallb_true_iff in H1.
           assert (negb (occursFreeIn_tm (chi sigma (all_form v f)) (substitute_vr sigma x)) = true).
-          { apply H1; apply the_rule_of_getFreeVars_form; simpl; destruct (vr_eq_dec x v).
-            - contradiction.
-            - tauto. 
+          { apply H1.
+            apply the_rule_of_getFreeVars_form.
+            simpl.
+            destruct (vr_eq_dec x v)...
           }
-          rewrite H0 in H2; inversion H2.
-        + reflexivity.
+          rewrite H0 in H2.
+          inversion H2.
+      }
     }
+    firstorder.
 Qed.
 
 Lemma substitute_tm_make_numeral :
   forall n : nat,
   forall sigma : substitution,
   substitute_tm sigma (make_numeral n) = make_numeral n.
-Proof.
-  intros n; induction n.
-  - intros sigma; simpl; reflexivity.
-  - intros sigma; simpl; rewrite (IHn sigma); reflexivity.
+Proof with eauto.
+  induction n; simpl...
+  intros sigma.
+  rewrite (IHn sigma)...
 Qed.
 
 Ltac simpl_eval_tm_make_numeral :=
@@ -880,10 +906,8 @@ Lemma occursFreeIn_tm_make_numeral :
   forall val : nat,
   forall x : vr,
   occursFreeIn_tm x (make_numeral val) = false.
-Proof.
-  intros val; induction val.
-  - intros x; simpl; reflexivity.
-  - intros x; simpl; rewrite (IHval x); reflexivity.
+Proof with eauto.
+  induction val; simpl...
 Qed.
 
 Ltac simplify_make_numeral := repeat (rewrite substitute_tm_make_numeral); repeat (apply occursFreeIn_tm_make_numeral).
@@ -894,15 +918,9 @@ Lemma vr_eq_dec_is_Nat_eq_dec {A : Type} :
   forall z1 : vr,
   forall z2 : vr,
   (if vr_eq_dec z1 z2 then x1 else x2) = (if Nat.eq_dec z1 z2 then x1 else x2).
-Proof.
+Proof with firstorder.
   intros x1 x2 z1 z2.
-  destruct (vr_eq_dec z1 z2).
-  - destruct (Nat.eq_dec z1 z2).
-    + reflexivity.
-    + contradiction.
-  - destruct (Nat.eq_dec z1 z2).
-    + contradiction.
-    + reflexivity.
+  destruct (vr_eq_dec z1 z2); destruct (Nat.eq_dec z1 z2)...
 Qed.
 
 Ltac eval_vr_eq_dec :=
@@ -911,6 +929,10 @@ Ltac eval_vr_eq_dec :=
 
 Ltac eval_in_vr_eq_dec H :=
   repeat (rewrite vr_eq_dec_is_Nat_eq_dec in H; simpl in H)
+.
+
+Ltac auto_show_it_is_sentence :=
+  tryif (apply orb_false_iff; constructor) then auto_show_it_is_sentence else (eval_vr_eq_dec; simplify_make_numeral)
 .
 
 Fixpoint relation_of_arity (n : nat) : Type :=
@@ -949,17 +971,20 @@ Fixpoint express_relation (n : nat) : form -> relation_of_arity n -> Prop :=
 
 Example express_relation_example1 :
   express_relation 2 (leq_form (ivar_tm 0) (ivar_tm 1)) (fun x0 : nat => fun x1 : nat => x0 <= x1).
-Proof.
-  simpl; intros val1 val2; constructor.
-  - intros x; apply orb_false_iff; constructor.
-    + eval_vr_eq_dec; simplify_make_numeral.
-    + eval_vr_eq_dec; simplify_make_numeral.
-  - constructor.
+Proof with eauto.
+  simpl.
+  intros val1 val2.
+  split.
+  - intros x.
+    auto_show_it_is_sentence.
+  - split.
     + intros H va.
-      eval_vr_eq_dec; simpl_eval_tm_make_numeral; tauto.
+      eval_vr_eq_dec.
+      simpl_eval_tm_make_numeral...
     + intros H.
       assert (H0 := H (fun _ : vr => 0)).
-      eval_in_vr_eq_dec H0; simpl_in_eval_tm_make_numeral H0; tauto.
+      eval_in_vr_eq_dec H0.
+      simpl_in_eval_tm_make_numeral H0...
 Qed.
 
 Fixpoint function_of_arity (n : nat) : Type :=
@@ -997,21 +1022,23 @@ Fixpoint express_function (n : nat) : form -> function_of_arity n -> Prop :=
     forall val : nat, express_function n' (substitute_form [(n, make_numeral val)] f) (lift_function n' func val)
   end
 .
-Ltac auto_show_it_is_sentence :=
-  tryif (apply orb_false_iff; constructor) then auto_show_it_is_sentence else (eval_vr_eq_dec; simplify_make_numeral)
-.
 
 Example express_function_example1 :
   express_function 3 (eqn_form (ivar_tm 0) (plus_tm (ivar_tm 1) (plus_tm (ivar_tm 2) (ivar_tm 3)))) (fun x1 : nat => fun x2 : nat => fun x3 : nat => x1 + (x2 + x3)).
-Proof.
-  simpl; intros val3 val2 val1 val0; constructor.
-  - intros x; auto_show_it_is_sentence.
-  - constructor.
+Proof with eauto.
+  simpl.
+  intros val3 val2 val1 val0.
+  split.
+  - intros x.
+    auto_show_it_is_sentence.
+  - split.
     + intros H va.
-      eval_vr_eq_dec; simpl_eval_tm_make_numeral; tauto.
+      eval_vr_eq_dec.
+      simpl_eval_tm_make_numeral...
     + intros H.
       assert (H0 := H (fun _ : vr => 0)).
-      eval_in_vr_eq_dec H0; simpl_in_eval_tm_make_numeral H0; tauto.
+      eval_in_vr_eq_dec H0.
+      simpl_in_eval_tm_make_numeral H0...
 Qed.
 
 End Chapter2.
